Proof of CminorSelect phase, modulo the fact that CompCert turns some external functions into builtins here, which violates atExternal axiom etc. Maybe this issue can be solved by understanding this inlining as linking, followed by internal inlining?
Added various CompCert backend files, and README that 
points out licensing issues of these.

sepcomp/effect_properties.v
@@ -16,6 +16,145 @@ Require Import sepcomp.effect_semantics.
 Require Import sepcomp.StructuredInjections.
 Require Import sepcomp.effect_simulations.
 
+Lemma FreeEffect_validblock: forall m lo hi sp b ofs
+        (EFF: FreeEffect m lo hi sp b ofs = true),
+      Mem.valid_block m b.
+Proof. intros.
+  unfold FreeEffect in EFF.
+  destruct (valid_block_dec m b); trivial; inv EFF.
+Qed.
+
+Lemma StoreEffectD: forall vaddr v b ofs
+      (STE: StoreEffect vaddr v b ofs = true),
+      exists i, vaddr = Vptr b i /\
+        (Int.unsigned i) <= ofs < (Int.unsigned i + Z.of_nat (length v)).
+Proof. intros.
+  unfold StoreEffect in STE. destruct vaddr; inv STE.
+  destruct (eq_block b0 b); inv H0.
+  exists i.
+  destruct (zle (Int.unsigned i) ofs); inv H1.
+  destruct (zlt ofs (Int.unsigned i + Z.of_nat (length v))); inv H0.
+  intuition.
+Qed.
+
+Lemma StoreEffect_PropagateLeft: forall chunk m vaddr v m'
+          (ST: Mem.storev chunk m vaddr v = Some m')
+          mu m2 (WD: SM_wd mu) (INJ : Mem.inject (as_inj mu) m m2)
+          vaddr' 
+          (VINJ : val_inject (restrict (as_inj mu) (vis mu)) vaddr vaddr')
+          v' m2' (ST2: Mem.storev chunk m2 vaddr' v' = Some m2')
+          b2 ofs 
+          (EFF : StoreEffect vaddr' (encode_val chunk v') b2 ofs = true)
+          (LBT2: locBlocksTgt mu b2 = false),
+      exists b1 delta, foreign_of mu b1 = Some (b2, delta) /\
+          StoreEffect vaddr (encode_val chunk v) b1 (ofs - delta) = true /\
+          Mem.perm m b1 (ofs - delta) Max Nonempty.
+Proof. intros.
+      apply StoreEffectD in EFF. destruct EFF as [i [VADDR' Hoff]]. subst.
+        simpl in ST2. inv VINJ. Focus 2. inv ST.
+      destruct (restrictD_Some _ _ _ _ _ H2); clear H2.
+      exists b1, delta.
+      split. destruct (joinD_Some _ _ _ _ _ H) as [EXT | [EXT LOC]]; clear H.
+             unfold vis in H0.
+             destruct (extern_DomRng' _ WD _ _ _ EXT) as [_ [_ [? _]]].
+             rewrite H in H0. simpl in H0.
+             destruct (frgnSrc _ WD _ H0) as [bb [dd [FF FT]]].
+             rewrite (foreign_in_extern _ _ _ _ FF) in EXT. inv EXT.
+             trivial.
+          destruct (local_DomRng _ WD _ _ _ LOC).
+            congruence.
+      rewrite encode_val_length in Hoff. rewrite <- size_chunk_conv in Hoff.
+      assert (Arith: Int.unsigned ofs1 <= ofs - delta < Int.unsigned ofs1 + size_chunk chunk).
+         assert (DD: delta >= 0 /\ 0 <= Int.unsigned ofs1 + delta <= Int.max_unsigned).
+                 eapply INJ. apply H. left.
+                 apply Mem.store_valid_access_3 in ST.
+                 eapply Mem.perm_implies. eapply Mem.valid_access_perm. eassumption. constructor.
+         destruct DD as [DD1 DD2].
+         specialize (Int.unsigned_range ofs1); intros I.
+         assert (URdelta: Int.unsigned (Int.repr delta) = delta).
+            apply Int.unsigned_repr. split. omega. omega.
+
+         rewrite Int.add_unsigned in Hoff. rewrite URdelta in Hoff.
+         rewrite (Int.unsigned_repr _ DD2) in Hoff. omega.
+
+      split. unfold StoreEffect.
+        destruct (eq_block b1 b1); try congruence. simpl; clear e.
+        destruct Arith. rewrite encode_val_length . rewrite <- size_chunk_conv.
+        destruct (zle (Int.unsigned ofs1) (ofs - delta)); try omega.
+          destruct (zlt (ofs - delta) (Int.unsigned ofs1 + size_chunk chunk)); try omega. trivial.
+      apply Mem.store_valid_access_3 in ST. 
+            eapply Mem.perm_implies. 
+            eapply Mem.perm_max. eapply ST. eassumption. constructor.
+Qed.
+
+Lemma free_free_inject : forall f m1 m1' m2 b1 lo hi b2 d m2'
+       (INJ: Mem.inject f m1 m2) 
+       (FREE1: Mem.free m1 b1 lo hi = Some m1')
+       (FREE2: Mem.free m2 b2 (lo+d) (hi+d) = Some m2')
+       (B: f b1 = Some(b2,d)),
+      Mem.inject f m1' m2'.
+Proof. intros.
+       eapply Mem.free_inject with (l:=(b1,lo,hi)::nil); try eassumption.
+       simpl. rewrite FREE1. trivial.
+       intros.
+          destruct (eq_block b0 b1); subst. rewrite H in B. inv B.
+            exists lo, hi. intuition.
+          assert (P1: Mem.perm m1 b0 ofs Max Nonempty).
+            eapply Mem.perm_implies. eapply Mem.perm_max; eassumption. apply perm_any_N.
+          assert (PM: Mem.perm m1 b1 (ofs - d + delta) Max Nonempty).
+            eapply Mem.perm_implies. eapply Mem.perm_max. 
+              eapply (Mem.free_range_perm _ _ _ _ _ FREE1). omega.
+              constructor.
+          exfalso.
+          destruct (Mem.mi_no_overlap _ _ _ INJ b0 _ _ _ _ _ _ _ n 
+               H B P1 PM) as [X | X]; apply X; trivial. omega.
+Qed.
+
+Lemma free_free_inject_same_block : forall f m1 m1' m2 b lo hi m2'
+       (INJ: Mem.inject f m1 m2) 
+       (FREE1: Mem.free m1 b lo hi = Some m1')
+       (FREE2: Mem.free m2 b lo hi = Some m2')
+       (B: f b = Some(b,0)),
+      Mem.inject f m1' m2'.
+Proof. intros. eapply free_free_inject; try eassumption.
+   repeat rewrite Zplus_0_r. trivial. 
+Qed.
+
+Lemma FreeEffect_PropagateLeft: forall
+   m sp lo hi m'
+   (FREE : Mem.free m sp lo hi = Some m')
+   mu m2 (SMV : sm_valid mu m m2)
+   (WD: SM_wd mu) spb'
+   (AI: as_inj mu sp = Some (spb', 0))
+   (VIS : vis mu sp = true) b2 ofs
+   (EFF : FreeEffect m2 lo hi spb' b2 ofs = true)
+   (LB: locBlocksTgt mu b2 = false),
+  exists b1 delta,
+    foreign_of mu b1 = Some (b2, delta) /\
+    FreeEffect m lo hi sp b1 (ofs - delta) = true /\
+    Mem.perm m b1 (ofs - delta) Max Nonempty.
+Proof. intros.
+      unfold FreeEffect in EFF.
+        destruct (valid_block_dec m2 b2); inv EFF.
+        destruct (eq_block b2 spb'); simpl in *; inv H0.
+        exists sp, 0. rewrite Zminus_0_r.
+        split. unfold vis in VIS.
+               destruct (joinD_Some _ _ _ _ _ AI) as [EXT | [NEXT LOC]]; clear H1.
+                 assert (LSP: locBlocksSrc mu sp = false). eapply (extern_DomRng' _ WD _ _ _ EXT).
+                 rewrite LSP in *. simpl in VIS. 
+                 destruct (frgnSrc _ WD _ VIS) as [bb2 [dd [F1 F2]]].
+                   rewrite (foreign_in_extern _ _ _ _ F1) in EXT. inv EXT. apply F1.
+               destruct (local_DomRng _ WD _ _ _ LOC); congruence.
+        split. unfold FreeEffect. 
+               destruct (valid_block_dec m sp).
+                 destruct (eq_block sp sp); trivial. elim n; trivial.
+               elim n; clear n. apply SMV. eapply as_inj_DomRng; eassumption.
+        eapply Mem.perm_implies. eapply Mem.perm_max. 
+           eapply (Mem.free_range_perm _ _ _ _ _ FREE).
+              destruct (zle lo ofs); simpl in H1; try discriminate.
+              destruct (zlt ofs hi); try discriminate. split; trivial.
+             constructor.
+Qed.
 
 (***** Some results on meminj_preserves_globals and variants of 
         LSR-clause match_genv  ************************************)
@@ -953,6 +1092,43 @@ Proof. intros m R L.
       subst. apply (Hzz3 _ _ H H1).
 Qed. 
 
+Lemma getsetVptr: forall z bb off n M v chunk k
+      (GET : ZMap.get ((Z.of_nat k) + z) 
+             (Mem.setN (encode_val chunk v) z M) = Pointer bb off n)
+      (HK: (k < (size_chunk_nat chunk))%nat), 
+     exists ofs, v=Vptr bb ofs.
+Proof. intros z bb off n M v chunk.
+destruct chunk. simpl in *.
+intros.
+Admitted.
+(* 
+induction k. 
+  simpl. rewrite ZMap.gss. intros; congruence.
+rewrite ZMap.gsspec; intros.
+  destruct (ZIndexed.eq (Z.of_nat (S k) + z) z). inv GET. 
+  simpl. ZIndexed.eq zz (Int.unsigned i)). inv H4. omega.
+                destruct (ZIndexed.eq zz (Int.unsigned i)). inv H4. omega.
+                destruct (ZIndexed.eq zz (Int.unsigned i+1)). inv H4.
+                  rewrite ZMap.gsspec in H4.
+ 
+  
+
+ unfold Z.of_nat in GET. simpl in *.
+rewrite Mem.setN_outside in GET. admit.
+  bb off n M i N.
+ induction N; simpl.
+   intros. inv HK.
+ intros k.
+ induction k; simpl in *; intros.
+      simpl in *. rewrite ZMap.gss in GET.
+  unfld Mem.setN in GET.
+  destruct (zlt zz (Int.unsigned i + Z.of_nat N)).
+   
+  rewrite ZMap.gsspec in GET.
+                  destruct (ZIndexed.eq zz (Int.unsigned i)). inv H4. omega.
+           *)  
+
+
 Lemma REACH_Store: forall m chunk b i v m'
      (ST: Mem.store chunk m b (Int.unsigned i) v = Some m')
      Roots (VISb: Roots b = true)
@@ -980,14 +1156,42 @@ destruct (eq_block r b); subst.
   remember (rev M) as rm.
   destruct rm; simpl in *. destruct HM as [zz [Hzz1 [Hzz2 Hzz3]]].
         inv Hzz1.
-        assert (v = Vptr bb off). 
-          rewrite (Mem.store_mem_contents _ _ _ _ _ _ ST) in H4. clear ST IHM H1.
+        intuition. 
+        assert (M= nil). destruct M; trivial. 
+             assert (@length (block * Z) nil = length (rev (p :: M))). rewrite Heqrm; trivial.
+             rewrite rev_length in H3. simpl in H3. inv H3.
+        subst. simpl in *. clear H Heqrm H0 H1.
+          rewrite (Mem.store_mem_contents _ _ _ _ _ _ ST) in H4. 
+          apply Mem.store_valid_access_3 in ST. destruct ST as [RP ALGN].
           rewrite PMap.gss in H4.
-        subst. admit. (*This is slightly wrong - the zz and v are not necessary aligned, 
-                        I think (also, zz may be entierly outside the region affected by the store operation *)
-        eexists. 
-           apply reach_nil. apply VISv. apply getBlocks_char. 
-              exists off. left.  trivial. 
+          destruct (zlt zz (Int.unsigned i)).
+            rewrite Mem.setN_outside in H4.
+            eexists. eapply reach_cons; try eassumption.
+                     apply reach_nil. assumption.
+            left; trivial. 
+          destruct (zlt zz ((Int.unsigned i) + Z.of_nat (length (encode_val chunk v)))).
+          Focus 2.
+            rewrite Mem.setN_outside in H4.
+            eexists. eapply reach_cons; try eassumption.
+                     apply reach_nil. assumption.
+            right; trivial.
+          rewrite encode_val_length in *. rewrite <- size_chunk_conv in *.
+          cut (exists ofs, v = Vptr bb ofs).
+             intros [ofs V]. subst. rewrite VISv in HeqRb. discriminate.
+             rewrite getBlocks_char. exists ofs; left. trivial.             
+          clear VISv Hzz3 H2 HeqRb Rr RP m'.
+          rewrite size_chunk_conv in l.
+         remember ((Mem.mem_contents m) !! b) as M. clear HeqM.
+(*          destruct v; simpl in *; try (eexists; reflexivity).
+          (*Undef*)*)
+           assert (exists k, zz = Z.of_nat k + Int.unsigned i).
+             assert (exists zn, zz = zn + Int.unsigned i /\ 0<=zn).
+               exists (zz-Int.unsigned i). omega.
+             destruct H as [? [? ?]]. destruct (Z_of_nat_complete _ H0).
+             subst. exists x0; trivial.   
+           destruct H. subst.
+           apply (getsetVptr (Int.unsigned i) bb off n M v chunk x H4). 
+           omega.
   destruct HM as [zz [Hzz1 [Hzz2 Hzz3]]].
     subst.
     remember (Roots b') as q.
@@ -1054,4 +1258,581 @@ Proof.
     destruct (decode_val_pointer_inv _ _ _ _ LD); clear LD; subst.
     simpl in *.
     inv H0. eassumption. 
+Qed.
+
+Axiom AllocContentsUndef2: forall m1 lo hi m2 b
+      (ALLOC:Mem.alloc m1 lo hi = (m2, b)),
+     (Mem.mem_contents m2) !! b = ZMap.init Undef.
+Lemma AllocContentsUndef1: forall m1 lo hi m2 b
+      (ALLOC:Mem.alloc m1 lo hi = (m2, b)) z,
+     ZMap.get z (Mem.mem_contents m2) !! b = Undef.
+Proof. intros. rewrite (AllocContentsUndef2 _ _ _ _ _ ALLOC). apply ZMap.gi. Qed.
+
+(*The axiom can easily be proven in Memory.v, in section
+  ALLOC, but repeating the proof here doesn't work, evem if 
+  we do Opaque Mem.alloc. 
+Section ALLOC.
+
+Variable m1: mem.
+Variables lo hi: Z.
+Variable m2: mem.
+Variable b: Values.block.
+Hypothesis ALLOC: Mem.alloc m1 lo hi = (m2, b).
+
+Lemma AllocContentsUndef: (Mem.mem_contents m2) !! b = ZMap.init Undef.
+Proof.
+   injection ALLOC. intros. simpl in H0. subst.
+   simpl. rewrite PMap.gss. reflexivity.
+Qed.
+End ALLOC.
+*)
+
+(*The following 2 lemmas are from Cminorgenproof.v*)
+Lemma nextblock_storev:
+  forall chunk m addr v m',
+  Mem.storev chunk m addr v = Some m' -> Mem.nextblock m' = Mem.nextblock m.
+Proof.
+  unfold Mem.storev; intros. destruct addr; try discriminate. 
+  eapply Mem.nextblock_store; eauto.
+Qed.
+Lemma nextblock_freelist:
+  forall fbl m m',
+  Mem.free_list m fbl = Some m' ->
+  Mem.nextblock m' = Mem.nextblock m.
+Proof.
+  induction fbl; intros until m'; simpl.
+  congruence.
+  destruct a as [[b lo] hi]. 
+  case_eq (Mem.free m b lo hi); intros; try congruence.
+  transitivity (Mem.nextblock m0). eauto. eapply Mem.nextblock_free; eauto.
+Qed.
+Lemma perm_freelist:
+  forall fbl m m' b ofs k p,
+  Mem.free_list m fbl = Some m' ->
+  Mem.perm m' b ofs k p ->
+  Mem.perm m b ofs k p.
+Proof.
+  induction fbl; simpl; intros until p.
+  congruence.
+  destruct a as [[b' lo] hi]. case_eq (Mem.free m b' lo hi); try congruence.
+  intros. eauto with mem.
+Qed.
+
+
+Lemma store_freshloc: forall ch m addr v m' 
+         (ST: Mem.storev ch m addr v = Some m'),
+         freshloc m m' = fun b => false.
+Proof. intros.
+  extensionality b.
+  apply nextblock_storev in ST.
+  (*specialize (storev_valid_block_2 _ _ _ _ _ ST b); intros.
+  specialize (storev_valid_block_1 _ _ _ _ _ ST b); intros.*)
+  apply freshloc_charF.
+  unfold Mem.valid_block. rewrite ST. xomega.
+Qed.
+
+Lemma freshloc_alloc: forall m1 lo hi m2 b 
+      (ALLOC: Mem.alloc m1 lo hi = (m2, b)),
+      freshloc m1 m2 = fun bb => eq_block bb b.
+Proof. intros.
+  unfold freshloc. extensionality bb.
+  destruct (eq_block bb b); subst; simpl.
+    specialize (Mem.valid_new_block _ _ _ _ _ ALLOC).
+    apply Mem.fresh_block_alloc in ALLOC.
+    intros.
+    destruct (valid_block_dec m2 b); try contradiction; simpl.
+    destruct (valid_block_dec m1 b); try contradiction; trivial.
+  destruct (valid_block_dec m2 bb); simpl; trivial.
+    destruct (Mem.valid_block_alloc_inv _ _ _ _ _ ALLOC _ v); try contradiction.
+    destruct (valid_block_dec m1 bb); try contradiction; trivial.
+Qed.
+
+Lemma freshloc_free: forall m sp i n m' 
+      (F: Mem.free m sp i n = Some m'),
+      freshloc m m' = fun b => false.
+Proof. intros.
+  unfold freshloc. extensionality b.
+  remember (valid_block_dec m' b) as d'.
+  destruct d'; simpl; trivial; clear Heqd'.
+    apply (Mem.valid_block_free_2 _ _ _ _ _ F ) in v.
+    remember (valid_block_dec m b) as d.
+    destruct d; trivial. congruence.
+Qed.
+
+Lemma freshloc_free_list: forall m n m' 
+      (F: Mem.free_list m n = Some m'),
+      freshloc m m' = fun b => false.
+Proof. intros.
+  unfold freshloc. apply nextblock_freelist in F.
+  extensionality b.
+  remember (valid_block_dec m' b) as d'.
+  destruct d'; simpl; trivial; clear Heqd'.
+    remember (valid_block_dec m b) as d.
+    destruct d; trivial. unfold Mem.valid_block in *.
+    rewrite F in v. congruence.
+Qed.
+
+(*new lemma*)
+Lemma free_parallel_inject:
+  forall j (m1 m2 : mem) (b : block) (lo hi : Z) (m1' : mem) ,
+  Mem.inject j m1 m2 ->
+  Mem.free m1 b lo hi = Some m1' -> 
+  forall b2 d (J: j b = Some(b2,d)),
+    exists m2' : mem, Mem.free m2 b2 (lo+d) (hi+d) = Some m2' /\ 
+                Mem.inject j m1' m2'.
+Proof. intros.
+  destruct (Mem.range_perm_free m2 b2 (lo+d) (hi+d)) as [m2' Hm2'].
+    intros. intros off; intros. 
+    specialize (Mem.perm_inject _ _ _ _ _ _ (off-d) Cur Freeable J H). intros.
+    assert (off - d + d = off) by omega. rewrite H3 in H2.
+    apply H2. clear H2 H3.
+    eapply (Mem.free_range_perm _ _ _ _ _ H0). omega.
+  exists m2'; split; trivial.
+  eapply (Mem.free_inject _ _ ((b,lo,hi)::nil)); try eassumption.
+    simpl. rewrite H0. trivial.
+  intros.
+  destruct (eq_block b1 b); subst.
+    rewrite H1 in J; inv J. exists lo, hi; split. left; trivial. omega.
+  assert (P: Mem.perm m1 b (ofs + delta - d) Max Nonempty).
+    eapply Mem.perm_implies. 
+      eapply Mem.perm_max.
+      apply (Mem.free_range_perm _ _ _ _ _ H0). omega.
+    constructor.
+  assert (P1: Mem.perm m1 b1 ofs Max Nonempty).
+    eapply Mem.perm_implies. 
+      eapply Mem.perm_max. eassumption. eapply perm_any_N.
+  exfalso.
+  destruct (Mem.mi_no_overlap _ _ _ H b1 _ _ _ _ _ _ _ n H1 J P1 P)
+    as [X | X]; apply X; trivial. omega.
+Qed.
+
+Lemma REACH_closed_free: forall m1 b lo hi m2 
+       (F: Mem.free m1 b lo hi = Some m2) X
+       (RC: REACH_closed m1 X),
+      REACH_closed m2 X.
+Proof. intros.
+      red; intros. apply RC; clear RC. 
+          rewrite REACHAX in H. destruct H as [L HL].
+          generalize dependent b0.
+          induction L; simpl; intros; inv HL.
+            apply REACH_nil. assumption.
+          specialize (IHL _ H1); clear H1.
+            eapply REACH_cons; try eassumption.
+            eapply Mem.perm_free_3; eassumption. 
+            rewrite (Mem.free_result _ _ _ _ _ F) in H4.
+            apply H4.
+Qed.
+
+Definition alloc_right_sm (mu: SM_Injection) sp: SM_Injection :=
+  Build_SM_Injection (locBlocksSrc mu)
+                     (fun b => eq_block b sp || locBlocksTgt mu b) 
+                     (pubBlocksSrc mu) (pubBlocksTgt mu)
+                     (local_of mu)
+                     (extBlocksSrc mu) (extBlocksTgt mu)
+                     (frgnBlocksSrc mu) (frgnBlocksTgt mu) (extern_of mu).
+
+Lemma alloc_right_sm_wd: forall mu sp (WD: SM_wd mu)
+      (NEW1: DomTgt mu sp = false),
+      SM_wd (alloc_right_sm mu sp).
+Proof. intros. 
+econstructor; simpl in *; try solve [eapply WD].
+  intros. unfold DomTgt in NEW1.
+    apply orb_false_iff in NEW1.
+    destruct NEW1.
+    remember (eq_block b sp) as d.
+    destruct d; simpl in *; apply eq_sym in Heqd.
+      subst. right. assumption.
+      eapply WD.
+  intros.
+    destruct (local_DomRng _ WD _ _ _ H). intuition.
+  intros.
+    destruct (pubSrc _ WD _ H) as [bb [dd [PB PT]]].
+    rewrite H in *.
+    exists bb, dd. rewrite (pub_in_local _ _ _ _ PB).
+    split; trivial.
+  intros. rewrite H. destruct (frgnSrc _ WD _ H) as [bb [dd [FRG FT]]].
+       rewrite (foreign_in_extern _ _ _ _ FRG). exists bb, dd; split; trivial. 
+  intros. rewrite (pubBlocksLocalTgt _ WD _ H). intuition. 
+Qed.
+
+Lemma alloc_right_sm_locBlocksTgt: forall mu sp,
+  locBlocksTgt (alloc_right_sm mu sp) = fun b => eq_block b sp || locBlocksTgt mu b.
+Proof. intros. reflexivity. Qed.
+
+Lemma alloc_right_sm_DomSrc: forall mu sp,
+      DomSrc (alloc_right_sm mu sp) = DomSrc mu.
+Proof. intros. extensionality b. 
+  unfold DomSrc, alloc_right_sm; simpl. trivial.
+Qed. 
+
+Lemma alloc_right_sm_DomTgt: forall mu sp,
+      DomTgt (alloc_right_sm mu sp) = fun b => eq_block b sp || DomTgt mu b.
+Proof. intros. extensionality b. 
+  unfold DomTgt, alloc_right_sm; simpl.
+  rewrite <- orb_assoc. trivial.
+Qed.
+
+Lemma alloc_right_sm_as_inj: forall mu sp,
+      as_inj (alloc_right_sm mu sp) = as_inj mu.
+Proof. intros. unfold alloc_right_sm, as_inj; reflexivity. Qed.
+
+Lemma alloc_right_sm_intern_incr: forall mu sp,
+      intern_incr mu (alloc_right_sm mu sp).
+Proof. intros. red; intros. simpl. intuition. Qed. 
+
+
+Definition alloc_left_sm (mu: SM_Injection) b1 b2 delta: SM_Injection :=
+  Build_SM_Injection (fun b => eq_block b b1 || locBlocksSrc mu b)
+                     (locBlocksTgt mu) (*b2 is already in locBlocksTgt!*)
+                     (pubBlocksSrc mu) (pubBlocksTgt mu)
+                     (fun b => if eq_block b b1 then Some(b2, delta) 
+                               else local_of mu b)
+                     (extBlocksSrc mu) (extBlocksTgt mu)
+                     (frgnBlocksSrc mu) (frgnBlocksTgt mu) (extern_of mu).
+
+Lemma alloc_left_sm_wd: forall mu b1 b2 delta (WD: SM_wd mu)
+      (NEW1: DomSrc mu b1 = false) (NEW2: locBlocksTgt mu b2 = true),
+      SM_wd (alloc_left_sm mu b1 b2 delta).
+Proof. intros. 
+econstructor; simpl in *; try solve [eapply WD].
+  intros. apply orb_false_iff in NEW1.
+    remember (eq_block b b1) as d.
+    destruct d; simpl in *; apply eq_sym in Heqd.
+      subst. right. apply NEW1.
+      apply WD.
+  intros. 
+    remember (eq_block b0 b1) as d.
+      destruct d; simpl in *; apply eq_sym in Heqd. inv H. split; trivial.
+    apply (local_DomRng _ WD _ _ _ H). 
+  intros.
+    destruct (pubSrc _ WD _ H) as [bb [dd [PB PT]]].
+    rewrite H in *.
+    exists bb, dd.
+    remember (eq_block b0 b1) as d.
+      destruct d; simpl in *; apply eq_sym in Heqd.
+        subst. unfold DomSrc in NEW1.
+        rewrite (pubBlocksLocalSrc _ WD _ H) in NEW1. simpl in *. discriminate.
+      rewrite (pub_in_local _ _ _ _ PB).
+      split; trivial.
+  intros. rewrite H. destruct (frgnSrc _ WD _ H) as [bb [dd [FRG FT]]].
+       rewrite (foreign_in_extern _ _ _ _ FRG). exists bb, dd; split; trivial. 
+  (*intros. rewrite (pubBlocksLocalTgt _ WD _ H). intuition. *)
+Qed.
+
+Lemma alloc_left_sm_as_inj_same: forall mu b1 b2 delta (WD: SM_wd mu)
+      (NEW1: DomSrc mu b1 = false),
+      as_inj (alloc_left_sm mu b1 b2 delta) b1 = Some(b2,delta). 
+Proof. intros.
+  unfold as_inj, join; simpl.
+  remember (extern_of mu b1) as d.
+  destruct d; apply eq_sym in Heqd; simpl. destruct p.
+    destruct (extern_DomRng' _ WD _ _ _ Heqd). rewrite NEW1 in H0. intuition.
+  destruct (eq_block b1 b1); subst; trivial.
+    elim n. trivial.
+Qed.
+
+Lemma alloc_left_sm_as_inj_other: forall mu b1 b2 delta b (H: b<>b1),
+      as_inj (alloc_left_sm mu b1 b2 delta) b = as_inj mu b.
+Proof. intros.
+  unfold as_inj, join; simpl.
+  destruct (eq_block b b1); subst; trivial. elim H. trivial.
+Qed.
+
+Lemma alloc_left_sm_intern_incr: 
+      forall mu b1 b2 delta (H: as_inj mu b1 = None) (WD: SM_wd mu),
+      intern_incr mu (alloc_left_sm mu b1 b2 delta).
+Proof. intros.
+  specialize (local_in_all _ WD); intros.
+  red; intros. destruct mu; simpl in *.
+  intuition.
+  red; intros.
+  destruct (eq_block b b1); subst.
+     rewrite (H0 _ _ _ H1) in H. inv H.
+  assumption.
+Qed.
+
+Lemma alloc_left_sm_inject_incr: 
+      forall mu b1 b2 delta (H: as_inj mu b1 = None),
+      inject_incr (as_inj mu) (as_inj (alloc_left_sm mu b1 b2 delta)).
+Proof. intros.
+  red; intros.
+  destruct (eq_block b b1); subst. congruence.
+  rewrite alloc_left_sm_as_inj_other; trivial.
+Qed.
+
+Lemma alloc_DomSrc: forall mu m1 m2 (SMV: sm_valid mu m1 m2) lo hi m1' b1
+      (ALLOC: Mem.alloc m1 lo hi = (m1', b1)),
+      DomSrc mu b1 = false.
+Proof. intros.
+  remember (DomSrc mu b1) as d.
+  destruct d; trivial; apply eq_sym in Heqd.
+  apply Mem.fresh_block_alloc in ALLOC.
+  elim ALLOC. apply SMV. apply Heqd.
+Qed.
+
+Lemma alloc_left_sm_DomSrc: forall mu b1 b2 delta,
+      DomSrc (alloc_left_sm mu b1 b2 delta) = fun b => eq_block b b1 || DomSrc mu b.
+Proof. intros. extensionality b. 
+  unfold DomSrc, alloc_left_sm; simpl.
+  rewrite <- orb_assoc. trivial.
+Qed.
+
+Lemma alloc_left_sm_DomTgt: forall mu b1 b2 delta,
+      DomTgt (alloc_left_sm mu b1 b2 delta) = DomTgt mu.
+Proof. intros. reflexivity. Qed.
+
+Lemma REACH_closed_alloc_left_sm: forall m lo hi sp m'
+          (ALLOC : Mem.alloc m lo hi = (m', sp))
+          mu (RC: REACH_closed m (vis mu)) b' delta,
+      REACH_closed m' (vis (alloc_left_sm mu sp b' delta)).
+Proof.
+  red; intros.
+  unfold vis. simpl.
+  destruct (eq_block b sp); try subst b. trivial.
+  simpl.
+  apply RC. rewrite REACHAX in H. 
+  destruct H as [L HL].
+  generalize dependent b.
+  induction L; simpl; intros; inv HL.
+    apply REACH_nil.
+      unfold vis in H. simpl in H.
+      destruct (eq_block b sp); try subst b. elim n; trivial.
+      apply H.
+    destruct (eq_block b'0 sp); try subst b'0.
+      clear - ALLOC H2 H4 n. 
+      rewrite (AllocContentsUndef1 _ _ _ _ _ ALLOC) in H4. inv H4. 
+    specialize (IHL _ H1 n1); clear H1.
+      apply (Mem.perm_alloc_4 _ _ _ _ _ ALLOC) in H2; trivial. 
+      destruct (Mem.alloc_unchanged_on (fun bb zz => True)
+         _ _ _ _ _ ALLOC) as [UP UC].
+      rewrite UC in H4; trivial. 
+        eapply REACH_cons; eassumption. 
+Qed.
+
+Theorem alloc_left_mapped_sm_inject:
+  forall mu m1 m2 lo hi m1' b1 b2 delta (WD: SM_wd mu)
+        (SMV: sm_valid mu m1 m2) (RC: REACH_closed m1 (vis mu))
+        (Locb2: locBlocksTgt mu b2 = true),
+  Mem.inject (as_inj mu) m1 m2 ->
+  Mem.alloc m1 lo hi = (m1', b1) ->
+  Mem.valid_block m2 b2 ->
+  0 <= delta <= Int.max_unsigned ->
+  (forall ofs k p, Mem.perm m2 b2 ofs k p -> delta = 0 \/ 0 <= ofs < Int.max_unsigned) ->
+  (forall ofs k p, lo <= ofs < hi -> Mem.perm m2 b2 (ofs + delta) k p) ->
+  Mem.inj_offset_aligned delta (hi-lo) ->
+  (forall b delta' ofs k p,
+   as_inj mu b = Some (b2, delta') -> 
+   Mem.perm m1 b ofs k p ->
+   lo + delta <= ofs + delta' < hi + delta -> False) ->
+  exists mu',
+     Mem.inject (as_inj mu') m1' m2
+  /\ intern_incr mu mu'
+  /\ as_inj mu' b1 = Some(b2, delta)
+  /\ (forall b, b <> b1 -> as_inj mu' b = as_inj mu b)
+  /\ SM_wd mu' /\ sm_valid mu' m1' m2
+  /\ sm_locally_allocated mu mu' m1 m2 m1' m2 
+  /\ REACH_closed m1' (vis mu').
+Proof.
+  intros. inversion H.
+  assert (AIb: as_inj mu b1 = None). eauto with mem.
+  assert (DS:= alloc_DomSrc _ _ _ SMV _ _ _ _ H0).
+  set (mu' := alloc_left_sm mu b1 b2 delta).
+  assert (intern_incr mu mu').
+    red; unfold mu'; intros. simpl.
+    intuition.
+    red; intros. destruct (eq_block b b1). subst b.
+       apply (local_in_all _ WD) in H2. congruence.
+    auto.
+  assert (Mem.mem_inj (as_inj mu') m1 m2).
+    inversion mi_inj; constructor; eauto with mem.
+    unfold mu'; intros. destruct (eq_block b0 b1).
+      subst b0.
+      elim (Mem.fresh_block_alloc _ _ _ _ _ H0). eauto with mem.
+    rewrite alloc_left_sm_as_inj_other in H8; trivial.
+      eauto.
+    unfold mu'; simpl. intros. destruct (eq_block b0 b1).
+      subst b0.
+      elim (Mem.fresh_block_alloc _ _ _ _ _ H0).
+      eapply Mem.perm_valid_block with (ofs := ofs). apply H9. generalize (size_chunk_pos chunk); omega.
+    rewrite alloc_left_sm_as_inj_other in H8; trivial.
+      eauto.
+    unfold mu'; simpl; intros. destruct (eq_block b0 b1).
+      subst b0.
+      elim (Mem.fresh_block_alloc _ _ _ _ _ H0). eauto with mem.
+    rewrite alloc_left_sm_as_inj_other in H8; trivial.
+      apply memval_inject_incr with (as_inj mu); auto.
+      apply alloc_left_sm_inject_incr; assumption. 
+  exists mu'. split. constructor.
+(* inj *)
+  eapply Mem.alloc_left_mapped_inj; eauto. 
+  unfold mu'; simpl. rewrite alloc_left_sm_as_inj_same; trivial.
+(* freeblocks *)
+  unfold mu'; simpl; intros. destruct (eq_block b b1). subst b. 
+  elim H9. eauto with mem.
+  rewrite alloc_left_sm_as_inj_other; trivial.
+  eauto with mem.
+(* mappedblocks *)
+  unfold mu'; simpl; intros.
+  destruct (eq_block b b1). 
+    subst. rewrite alloc_left_sm_as_inj_same in H9; trivial.
+     congruence. eauto.
+  rewrite alloc_left_sm_as_inj_other in H9; trivial.
+    eauto.
+(* overlap *)
+  unfold mu'; red; intros.
+  exploit Mem.perm_alloc_inv. eauto. eexact H12. intros P1.
+  exploit Mem.perm_alloc_inv. eauto. eexact H13. intros P2.
+  destruct (eq_block b0 b1); try subst b0; destruct (eq_block b3 b1); try subst b3. 
+    elim H9; trivial.
+    rewrite alloc_left_sm_as_inj_same in H10; trivial.
+    inversion H10. subst b1' delta1.
+    rewrite alloc_left_sm_as_inj_other in H11; trivial. 
+    destruct (eq_block b2 b2'); auto. subst b2'. right; red; intros.
+    eapply H6; eauto. omega.
+  
+  rewrite alloc_left_sm_as_inj_same in H11; trivial. 
+    rewrite alloc_left_sm_as_inj_other in H10; trivial.
+    inversion H11. subst b2' delta2.
+    destruct (eq_block b1' b2); auto. subst b1'. right; red; intros.
+    eapply H6; eauto. omega.
+  rewrite alloc_left_sm_as_inj_other in H10; trivial.
+  rewrite alloc_left_sm_as_inj_other in H11; trivial.
+  eauto.
+(* representable *)
+  unfold mu'; intros.
+  destruct (eq_block b b1).
+   subst. 
+    rewrite alloc_left_sm_as_inj_same in H9; trivial.
+    injection H9; intros; subst b' delta0. clear H9; destruct H10.
+    exploit Mem.perm_alloc_inv; eauto; rewrite dec_eq_true; intro.
+    exploit H3. apply H4 with (k := Max) (p := Nonempty); eauto.
+    generalize (Int.unsigned_range_2 ofs). omega.
+   exploit Mem.perm_alloc_inv; eauto; rewrite dec_eq_true; intro.
+   exploit H3. apply H4 with (k := Max) (p := Nonempty); eauto.
+   generalize (Int.unsigned_range_2 ofs). omega.
+  rewrite alloc_left_sm_as_inj_other in H9; trivial.
+  eapply mi_representable; try eassumption.
+  destruct H10; eauto using Mem.perm_alloc_4.
+(* incr *)
+  split. auto.
+(* image of b1 *)
+  split. unfold mu'; simpl.
+    rewrite alloc_left_sm_as_inj_same; trivial.
+(* image of others *)
+  split. intros. unfold mu'; simpl.
+  rewrite alloc_left_sm_as_inj_other; trivial.
+(* SM_wd*)
+  split. unfold mu'. eapply alloc_left_sm_wd; try eassumption.
+ (* sm_valid*)
+  split. red.
+  split; intros. unfold mu' in H9; simpl in H9.
+    unfold DOM, DomSrc in H9; simpl in H9.
+    destruct (eq_block b0 b1); try subst b0.
+      apply (Mem.valid_new_block _ _ _ _ _ H0).
+    simpl in H9.
+    apply (Mem.valid_block_alloc _ _ _ _ _ H0).
+    apply SMV. apply H9.
+  unfold mu' in H9; simpl in H9. unfold RNG, DomTgt in H9; simpl in H9.
+    destruct (eq_block b0 b2); try subst b0.
+      assumption.
+    simpl in H9.
+    apply SMV. apply H9.
+(*sm_locally_allocated*)
+  split. apply sm_locally_allocatedChar. unfold mu'; simpl.
+  repeat split; extensionality bb; 
+   try rewrite (freshloc_irrefl m2); 
+   try rewrite (freshloc_alloc _ _ _ _ _ H0); simpl. 
+  unfold DomSrc; simpl. rewrite <- orb_assoc. rewrite orb_comm. trivial.
+  unfold DomTgt; simpl. destruct (eq_block bb b2); try subst bb; simpl.
+    rewrite Locb2. trivial.
+    intuition.
+  intuition.
+  destruct (eq_block bb b2); try subst bb; simpl.
+    rewrite Locb2. trivial.
+  intuition.
+(* REACH_closed*)
+  clear - RC H0.
+  eapply REACH_closed_alloc_left_sm; eassumption.
+Qed.
+
+Lemma genv_find_add_globals_fresh: forall {F V} defs (g:Genv.t F V) i
+  (G: ~ In i (map fst defs)), 
+  Genv.find_symbol (Genv.add_globals g defs) i =  Genv.find_symbol g i.
+Proof. intros F V defs.
+  induction defs; simpl; intros. trivial.
+  destruct a.
+  rewrite IHdefs. 
+    unfold Genv.find_symbol, Genv.genv_symb. simpl. rewrite PTree.gso. reflexivity.
+    intros N. apply G; left. subst; simpl; trivial.
+  intros N. apply G; right; trivial.
+Qed.
+
+Lemma add_globals_find_symbol: forall {F V} (defs : list (ident * globdef F V)) 
+    (R: list_norepet (map fst defs)) (g: Genv.t F V) m0 m 
+    (G: Genv.alloc_globals (Genv.add_globals g defs) m0 defs = Some m)
+    (N: Genv.genv_next g = Mem.nextblock m0)
+    b (VB: Mem.valid_block m b),
+    Mem.valid_block m0 b \/ 
+    exists id, Genv.find_symbol (Genv.add_globals g defs) id = Some b.
+Proof. intros F V defs.
+induction defs; simpl; intros.
+  inv G. left; trivial.
+remember (Genv.alloc_global (Genv.add_globals (Genv.add_global g a) defs) m0 a) as d.
+  destruct d; inv G. apply eq_sym in Heqd.
+  inv R.
+  specialize (IHdefs H3 _ _ _ H0). simpl in *.
+  rewrite N in *.
+  assert (P: Pos.succ (Mem.nextblock m0) = Mem.nextblock m1).
+    clear IHdefs N VB H0.
+    rewrite (@Genv.alloc_global_nextblock _ _ _ _ _ _ Heqd). trivial.
+  destruct (IHdefs P _ VB); try (right; assumption).
+  clear IHdefs P VB H0.
+  destruct a. destruct g0. simpl in Heqd.
+   remember (Mem.alloc m0 0 1) as t.
+   destruct t; inv Heqd. apply eq_sym in Heqt.
+   apply (Mem.drop_perm_valid_block_2 _ _ _ _ _ _ H1) in H. clear H1.
+   apply (Mem.valid_block_alloc_inv _ _ _ _ _ Heqt) in H. 
+   destruct H; subst; try (left; assumption).
+     right. apply Mem.alloc_result in Heqt. subst.
+     exists i. rewrite genv_find_add_globals_fresh; trivial.
+     unfold Genv.find_symbol, Genv.genv_symb. simpl.
+     rewrite PTree.gss. rewrite N. trivial. 
+simpl in *. 
+  remember (Mem.alloc m0 0 (Genv.init_data_list_size (gvar_init v))) as t.
+  destruct t; inv Heqd. apply eq_sym in Heqt.
+  remember (store_zeros m2 b0 0 (Genv.init_data_list_size (gvar_init v))) as q.
+  destruct q; inv H1. apply eq_sym in Heqq.
+  remember (Genv.store_init_data_list
+         (Genv.add_globals (Genv.add_global g (i, Gvar v)) defs) m3 b0 0
+         (gvar_init v)) as w.
+  destruct w; inv H4. apply eq_sym in Heqw.
+  apply (Mem.drop_perm_valid_block_2 _ _ _ _ _ _ H1) in H. clear H1.
+  assert (VB3: Mem.valid_block m3 b). unfold Mem.valid_block.
+    rewrite <- (@Genv.store_init_data_list_nextblock _ _ _ _ _ _ _ _ Heqw).
+    apply H.
+  clear H Heqw.
+  assert (VB2: Mem.valid_block m2 b). unfold Mem.valid_block.
+    rewrite <- (@Genv.store_zeros_nextblock _ _ _ _ _ Heqq).
+    apply VB3.
+  clear VB3 Heqq.
+  apply (Mem.valid_block_alloc_inv _ _ _ _ _ Heqt) in VB2. 
+   destruct VB2; subst; try (left; assumption).
+     right. apply Mem.alloc_result in Heqt. subst.
+     exists i. rewrite genv_find_add_globals_fresh; trivial.
+     unfold Genv.find_symbol, Genv.genv_symb. simpl.
+     rewrite PTree.gss. rewrite N. trivial. 
+Qed.
+
+Lemma valid_init_is_global :
+  forall {F V} (prog:AST.program F V)
+         (R: list_norepet (map fst (prog_defs prog)))
+  m (G: Genv.init_mem prog = Some m)  
+  b (VB: Mem.valid_block m b), 
+  exists id, Genv.find_symbol (Genv.globalenv prog) id = Some b.
+Proof. intros.
+  unfold Genv.init_mem, Genv.globalenv in G. simpl in *.
+  destruct (add_globals_find_symbol _ R (@Genv.empty_genv _ _ ) _ _ G (eq_refl _) _ VB)
+    as [VBEmpty | X]; trivial.
+  exfalso. clear - VBEmpty. unfold Mem.valid_block in VBEmpty.
+    rewrite Mem.nextblock_empty in VBEmpty. xomega.
 Qed.
