sepcomp/CminorSel_coop.v
@@ -1,0 +1,260 @@
+Require Import Coqlib.
+Require Import AST.
+Require Import Integers.
+Require Import compcert.common.Values.
+Require Import Memory.
+Require Import Events.
+Require Import Globalenvs.
+
+Require Import sepcomp.CminorSel. 
+Require Import sepcomp.mem_lemmas. (*for mem_forward*)
+Require Import sepcomp.core_semantics.
+
+(*Require Import Maps.
+Require Import Cminor.
+Require Import Op.
+Require Import Switch.
+Require Import Smallstep.*)
+
+Inductive CMinSel_core: Type :=
+  | CMinSel_State:                      (**r execution within a function *)
+      forall (f: function)              (**r currently executing function  *)
+             (s: stmt)                  (**r statement under consideration *)
+             (k: cont)                  (**r its continuation -- what to do next *)
+             (sp: val)                  (**r current stack pointer *)
+             (e: Cminor.env),           (**r current local environment *)
+      CMinSel_core
+  | CMinSel_Callstate:                  (**r invocation of a fundef  *)
+      forall (f: fundef)                (**r fundef to invoke *)
+             (args: list val)           (**r arguments provided by caller *)
+             (k: cont),                 (**r what to do next  *)
+      CMinSel_core
+  | CMinSel_Returnstate:
+      forall (v: val)                   (**r return value *)
+             (k: cont),                 (**r what to do next *)
+      CMinSel_core.
+
+Definition ToState (q:CMinSel_core) (m:mem): CminorSel.state :=
+  match q with 
+     CMinSel_State f s k sp e => State f s k sp e m
+   | CMinSel_Callstate f args k => Callstate f args k m
+   | CMinSel_Returnstate v k => Returnstate v k m 
+  end.
+
+Definition FromState (c: CminorSel.state) : CMinSel_core * mem :=
+  match c with 
+     State f s k sp e m => (CMinSel_State f s k sp e, m)
+   | Callstate f args k m => (CMinSel_Callstate f args k, m)
+   | Returnstate v k m => (CMinSel_Returnstate v k, m)
+  end. 
+
+Definition CMinSel_at_external (c: CMinSel_core) : option (external_function * signature * list val) :=
+  match c with
+  | CMinSel_State _ _ _ _ _ => None
+  | CMinSel_Callstate fd args k => match fd with
+                                  Internal f => None
+                                | External ef => Some (ef, ef_sig ef, args)
+                              end
+  | CMinSel_Returnstate v k => None
+ end.
+
+Definition CMinSel_after_external (vret: option val) (c: CMinSel_core) : option CMinSel_core :=
+  match c with 
+    CMinSel_Callstate fd args k => 
+         match fd with
+            Internal f => None
+          | External ef => match vret with
+                             None => Some (CMinSel_Returnstate Vundef k)
+                           | Some v => Some (CMinSel_Returnstate v k)
+                           end
+         end
+  | _ => None
+  end.
+
+Definition CMinSel_corestep (ge : genv)  (q : CMinSel_core) (m : mem) (q' : CMinSel_core) (m' : mem) : Prop.
+  destruct q; destruct q'.
+  (*State - State*)
+       apply (exists t, step ge (State f s k sp e m)  t (State f0 s0 k0 sp0 e0 m')).
+  (*State - Callstate: one case: step_call*)
+       apply (exists t, step ge (State f s k sp e m)  t (Callstate f0 args k0 m')).
+  (*State - Returnstate - three cases: step_skip_call, step_return_0, step_return_1*)
+       apply (exists t, step ge (State f s k sp e m)  t (Returnstate v k0 m')).
+  (*Callstate - State: only case: step_internal_function*)
+       apply (exists t, step ge (Callstate f args k m) t (State f0 s k0 sp e m')).
+  (*Callstate - Callstate: no case*)
+       apply False.
+  (*Callstate - Returnstate: one case: step_external_function : we don't want this as a step in this semantics, since
+                    stepping should not happen at_external*)
+       apply False.
+  (*Returnstate - State: one case: step_return*)
+       apply (exists t, step ge (Returnstate v k m) t (State f s k0 sp e m')).
+  (*Returnstate - Callstate: no case*)
+       apply False.
+  (*Returnstate - Returnstate: no case*)
+       apply False.
+Defined.
+
+Lemma CMinSel_corestep_not_at_external:
+       forall ge m q m' q', CMinSel_corestep ge q m q' m' -> CMinSel_at_external q = None.
+  Proof. intros.
+     unfold CMinSel_corestep in H. 
+     destruct q; destruct q'; simpl in *; try reflexivity.
+       (*case step_internal_function*)  
+             destruct H as [t Ht]. inversion Ht; subst. reflexivity.
+       (*Call - Call: no case*)
+             contradiction.
+       (*Call - Return: no case in CminorSel_corestep*)
+             contradiction.
+  Qed.
+
+Definition CMinSel_halted (q : CMinSel_core): option val :=
+    match q with 
+       CMinSel_Returnstate v Kstop => Some v
+     | _ => None
+    end.
+
+Lemma CMinSel_corestep_not_halted : forall ge m q m' q', 
+       CMinSel_corestep ge q m q' m' -> CMinSel_halted q = None.
+  Proof. intros.
+     unfold CMinSel_corestep in H. 
+     destruct q; destruct q'; simpl in *; try reflexivity.
+          (*case step_return*) 
+             destruct H as [t Ht]. inversion Ht; subst. 
+             destruct v; reflexivity.
+       (*Returnstate - Callstate: no case*)
+             contradiction.
+       (*Returnstate - Returnstate: no case in Cmin_corestep*)
+             contradiction.
+  Qed.
+    
+Lemma CMinSel_at_external_halted_excl :
+       forall q, CMinSel_at_external q = None \/ CMinSel_halted q = None.
+   Proof. intros. destruct q; auto. Qed.
+
+Lemma CMinSel_after_at_external_excl : forall retv q q',
+      CMinSel_after_external retv q = Some q' -> CMinSel_at_external q' = None.
+  Proof. intros.
+       destruct q; simpl in *; try inv H.
+       destruct f; try inv H1; simpl; trivial.
+         destruct retv; inv H0; simpl; trivial.
+Qed.
+
+Definition CMinSel_initial_core (ge:genv) (v: val) (args:list val): option CMinSel_core :=
+   match v with
+     | Vptr b i => 
+          if Int.eq_dec i Int.zero 
+          then match Genv.find_funct_ptr ge b with
+                 | None => None
+                 | Some f => Some (CMinSel_Callstate f args Kstop)
+               end
+          else None
+     | _ => None
+    end.
+
+Definition CMinSel_core_sem : CoreSemantics genv CMinSel_core mem.
+  eapply @Build_CoreSemantics with (at_external:=CMinSel_at_external)
+                  (after_external:=CMinSel_after_external)
+                  (corestep:=CMinSel_corestep)
+                  (halted:=CMinSel_halted). 
+    apply CMinSel_initial_core.
+    apply CMinSel_corestep_not_at_external.
+    apply CMinSel_corestep_not_halted.
+    apply CMinSel_at_external_halted_excl.
+    apply CMinSel_after_at_external_excl.
+Defined.
+
+
+Lemma CMinSel_corestep_2_CompCertStep: forall (ge : genv)  (q :CMinSel_core) (m : mem) (q' : CMinSel_core) (m' : mem) ,
+   CMinSel_corestep ge q m q' m' -> 
+   exists t, step ge (ToState q m) t (ToState q' m').
+Proof.
+  intros. destruct q; destruct q'; induction H; simpl; eauto. 
+Qed.
+
+Lemma CompCertStep_CMinSel_corestep: forall (ge : genv)  (q : CMinSel_core) (m : mem) (q' : CMinSel_core) (m' : mem)  t,
+   step ge (ToState q m) t (ToState q' m') ->
+   CMinSel_at_external q = None ->
+   CMinSel_corestep ge q m q' m'.
+Proof.
+  intros. destruct q; destruct q'; simpl in *; try eexists; try eassumption; inv H; discriminate.
+Qed.
+
+Lemma CompCertStep_CMinSel_corestep': forall (ge : genv)  (q : CMinSel_core) (m : mem) c' t q' m',
+   step ge (ToState q m) t c' ->
+   CMinSel_at_external q = None ->
+     q'= fst (FromState c') -> m' = snd (FromState c') -> 
+     CMinSel_corestep ge q m q' m'.
+Proof.
+  intros. assert (c' = ToState q' m'). subst. destruct c'; simpl; trivial.
+  rewrite H3 in H. clear H3. eapply CompCertStep_CMinSel_corestep; eassumption.
+Qed.
+
+Lemma CMinSel_forward : forall g c m c' m' (CS: CMinSel_corestep g c m c' m'), 
+      mem_lemmas.mem_forward m m'.
+  Proof. intros.
+     unfold CMinSel_corestep in CS. 
+     destruct c; destruct c'; simpl in *; try contradiction. 
+       destruct CS as [t CS].
+         inv CS; try apply mem_forward_refl.
+         (*Storev*)
+          destruct vaddr; simpl in H15; inv H15. 
+          eapply store_forward. eassumption. 
+         (*builtin*) 
+          eapply external_call_mem_forward; eassumption.
+       destruct CS as [t CS].
+         inv CS; simpl; try apply mem_forward_refl.
+         (*free*)
+         eapply free_forward; eassumption.
+       destruct CS as [t CS].
+         inv CS; simpl.
+         eapply free_forward; eassumption.
+         eapply free_forward; eassumption.
+         eapply free_forward; eassumption.
+       destruct CS as [t CS].
+         inv CS; simpl. 
+         eapply alloc_forward; eassumption.
+       destruct CS as [t CS].
+         inv CS; simpl. apply mem_forward_refl.
+Qed.
+
+Definition coopstep g c m c' m' :=
+   CMinSel_corestep g c m c' m'.
+
+Lemma cminsel_coopstep_not_at_external: forall ge m q m' q',
+  coopstep ge q m q' m' -> CMinSel_at_external q = None.
+Proof.
+  intros.
+  eapply CMinSel_corestep_not_at_external. apply H. 
+Qed.
+
+Lemma cminsel_coopstep_not_halted :
+  forall ge m q m' q', coopstep ge q m q' m' -> CMinSel_halted q = None.
+Proof.
+  intros.
+  eapply CMinSel_corestep_not_halted. apply H.
+Qed.
+
+Program Definition cminsel_core_sem : 
+  CoreSemantics genv CMinSel_core mem :=
+  @Build_CoreSemantics _ _ _ 
+    CMinSel_initial_core
+    CMinSel_at_external
+    CMinSel_after_external
+    CMinSel_halted
+    coopstep
+    cminsel_coopstep_not_at_external
+    cminsel_coopstep_not_halted 
+    CMinSel_at_external_halted_excl
+    CMinSel_after_at_external_excl.
+
+(************************NOW SHOW THAT WE ALSO HAVE A COOPSEM******)
+
+Lemma cminsel_coop_forward : forall g c m c' m' (CS: coopstep g c m c' m'), 
+      mem_lemmas.mem_forward m m'.
+Proof. intros. eapply CMinSel_forward. apply CS. Qed.
+
+Program Definition cminsel_coop_sem : 
+  CoopCoreSem genv CMinSel_core.
+apply Build_CoopCoreSem with (coopsem := cminsel_core_sem).
+  apply cminsel_coop_forward.
+Defined.
