sepcomp/Registers.v
@@ -1,0 +1,62 @@
+(* *********************************************************************)
+(*                                                                     *)
+(*              The Compcert verified compiler                         *)
+(*                                                                     *)
+(*          Xavier Leroy, INRIA Paris-Rocquencourt                     *)
+(*                                                                     *)
+(*  Copyright Institut National de Recherche en Informatique et en     *)
+(*  Automatique.  All rights reserved.  This file is distributed       *)
+(*  under the terms of the INRIA Non-Commercial License Agreement.     *)
+(*                                                                     *)
+(* *********************************************************************)
+
+(** Pseudo-registers and register states.
+
+  This library defines the type of pseudo-registers (also known as
+  "temporaries" in compiler literature) used in the RTL
+  intermediate language.  We also define finite sets and finite maps
+  over pseudo-registers. *)
+
+Require Import Coqlib.
+Require Import AST.
+Require Import Maps.
+Require Import Ordered.
+Require FSetAVL.
+
+Definition reg: Type := positive.
+
+Module Reg.
+
+Definition eq := peq.
+
+Definition typenv := PMap.t typ.
+
+End Reg.
+
+(** Mappings from registers to some type. *)
+
+Module Regmap := PMap.
+
+Set Implicit Arguments.
+
+Definition regmap_optget
+    (A: Type) (or: option reg) (dfl: A) (rs: Regmap.t A) : A :=
+  match or with
+  | None => dfl
+  | Some r => Regmap.get r rs
+  end.
+
+Definition regmap_optset
+    (A: Type) (or: option reg) (v: A) (rs: Regmap.t A) : Regmap.t A :=
+  match or with
+  | None => rs
+  | Some r => Regmap.set r v rs
+  end.
+
+Notation "a # b" := (Regmap.get b a) (at level 1).
+Notation "a ## b" := (List.map (fun r => Regmap.get r a) b) (at level 1).
+Notation "a # b <- c" := (Regmap.set b c a) (at level 1, b at next level).
+
+(** Sets of registers *)
+
+Module Regset := FSetAVL.Make(OrderedPositive).
